cleanup

code/kyber2/impl/Lib.Arithmetic.Sums.fst
@@ -2,6 +2,8 @@ module Lib.Arithmetic.Sums
 
 open FStar.Tactics.Typeclasses
 
+open FStar.Math.Lemmas
+
 open Lib.Arithmetic.Group
 open Lib.Arithmetic.Ring
 
@@ -9,7 +11,7 @@ open FStar.Math.Lemmas
 
 open Spec.Powtwo.Lemmas
 open FStar.Mul
-open FStar.UInt
+//open FStar.UInt
 open FStar.Seq
 open Lib.Sequence
 
@@ -46,25 +48,25 @@ let br_lemma_rec i x =
     assert(br 0 0 = 0);
     let v = UInt.to_vec #1 x in
     let vbr = Seq.createi 1 (fun p -> (Seq.index #_ #1 v (1-1-p))) in
-    assert_norm(from_vec #1 vbr == br 1 x);
+    assert_norm(UInt.from_vec #1 vbr == br 1 x);
     eq_intro #_ #1 v (BitVector.zero_vec #1);
     eq_intro #_ #1 v vbr;
-    zero_from_vec_lemma #1
+    UInt.zero_from_vec_lemma #1
     end
   else begin
   let v1:lseq bool i = UInt.to_vec #i x in
   let v1br = Seq.createi i (fun p -> (Seq.index #_ #i v1 (i-1-p))) in
-  assert(from_vec #i v1br == br i x);
+  assert(UInt.from_vec #i v1br == br i x);
   let v2:lseq bool (i+1) = UInt.to_vec #(i+1) x in
   let v2br = Seq.createi (i+1) (fun p -> (Seq.index #_ #(i+1) v2 ((i+1)-1-p))) in
-  assert_norm(from_vec #(i+1) v2br == br (i+1) x);
+  assert_norm(UInt.from_vec #(i+1) v2br == br (i+1) x);
   to_vec_equal_lemma i 1 x;
-  from_vec_propriety #(i+1) v2 1;
-  assert(from_vec #1 (slice v2 0 1) = 0);
-  zero_from_vec_lemma #1;
+  UInt.from_vec_propriety #(i+1) v2 1;
+  assert(UInt.from_vec #1 (slice v2 0 1) = 0);
+  UInt.zero_from_vec_lemma #1;
   assert(v2.[0] = false);
   assert(v2br.[i] = false);
-  from_vec_propriety #(i+1) v2br i;
+  UInt.from_vec_propriety #(i+1) v2br i;
   eq_intro v1br (Seq.sub v2br 0 i)
   end
 
@@ -76,10 +78,10 @@ let rec br_lemma_one (i:size_nat{i>0}) : Lemma (ensures br i 1 = pow2 (i-1)) (de
   if (i = 1) then
     let v = UInt.to_vec #1 1 in
     let vbr = Seq.createi 1 (fun p -> (Seq.index #_ #1 v (1-1-p))) in
-    assert_norm(from_vec #1 vbr == br 1 1);
+    assert_norm(UInt.from_vec #1 vbr == br 1 1);
     eq_intro #_ #1 v (BitVector.ones_vec #1);
     eq_intro #_ #1 v vbr;
-    ones_from_vec_lemma #1
+    UInt.ones_from_vec_lemma #1
   else
     (br_lemma_one (i-1); br_lemma_rec (i-1) 1)
 
@@ -92,30 +94,30 @@ let br_lemma_n2_1 i x =
   else begin
   let v0:lseq bool i = UInt.to_vec #i x in
   let v0br = Seq.createi i (fun p -> (Seq.index #_ #i v0 (i-1-p))) in
-  assert(from_vec #i v0br == br i x);
+  assert(UInt.from_vec #i v0br == br i x);
   let v1:lseq bool (i+1) = UInt.to_vec #(i+1) (x+pow2 i) in
   let v1br:lseq bool (i+1) = Seq.createi (i+1) (fun p -> (Seq.index #_ #(i+1) v1 ((i+1)-1-p))) in
-  assert_norm(from_vec #(i+1) v1br == br (i+1) (x+pow2 i));
+  assert_norm(UInt.from_vec #(i+1) v1br == br (i+1) (x+pow2 i));
   let v2:lseq bool (i+1) = UInt.to_vec #(i+1) x in
   let v2br:lseq bool (i+1) = Seq.createi (i+1) (fun p -> (Seq.index #_ #(i+1) v2 ((i+1)-1-p))) in
-  assert_norm(from_vec #(i+1) v2br == br (i+1) x);
+  assert_norm(UInt.from_vec #(i+1) v2br == br (i+1) x);
   to_vec_equal_lemma i 1 x;
-  from_vec_propriety #(i+1) v2 1;
-  zero_from_vec_lemma #1;
+  UInt.from_vec_propriety #(i+1) v2 1;
+  UInt.zero_from_vec_lemma #1;
   assert(v2br.[i] = false);
   eq_intro v0br (Seq.sub v2br 0 i);
-  from_vec_lemma_1 #i v0br (Seq.sub v2br 0 i);
+  UInt.from_vec_lemma_1 #i v0br (Seq.sub v2br 0 i);
   let v :lseq bool (i+1) = Seq.concat #_ #1 #i (BitVector.ones_vec #1) (Seq.sub v2 1 i) in
-  append_lemma #1 #i (BitVector.ones_vec #1) (Seq.sub v2 1 i);
-  assert(from_vec #(i+1) v == (x+pow2 i));
-  from_vec_lemma_1 #(i+1) v1 v;
+  UInt.append_lemma #1 #i (BitVector.ones_vec #1) (Seq.sub v2 1 i);
+  assert(UInt.from_vec #(i+1) v == (x+pow2 i));
+  UInt.from_vec_lemma_1 #(i+1) v1 v;
   Seq.Properties.lemma_append_inj (Seq.sub v1 0 1) (Seq.sub v1 1 i) (Seq.sub v 0 1) (Seq.sub v2 1 i);
-  from_vec_lemma_1 #1 (Seq.sub v1 0 1) (Seq.sub v 0 1);
+  UInt.from_vec_lemma_1 #1 (Seq.sub v1 0 1) (Seq.sub v 0 1);
   assert(v1br.[i] = true);
   eq_intro (Seq.sub v1br 0 i) (Seq.sub v2br 0 i);
-  from_vec_lemma_1 #i (Seq.sub v1br 0 i) (Seq.sub v2br 0 i);
-  from_vec_propriety #(i+1) v1br i;
-  assert(from_vec #1 (Seq.sub v1br i 1) == 1)
+  UInt.from_vec_lemma_1 #i (Seq.sub v1br 0 i) (Seq.sub v2br 0 i);
+  UInt.from_vec_propriety #(i+1) v1br i;
+  assert(UInt.from_vec #1 (Seq.sub v1br i 1) == 1)
   end
 
 let rec br_lemma_pow (i:size_nat{i>0}) (p:size_nat{p < i /\ pow2 p < pow2 i}) : Lemma (ensures br i (pow2 p) = pow2 (i-1-p)) (decreases i) =
@@ -161,26 +163,26 @@ let br_lemma_n2_2 i x =
 let br_lemma_div_even (i:size_nat{i>0}) (x:nat{x<pow2 i /\ x%2 = 0}) : Lemma (br i (x/2) = (2 * br i x) % pow2 i) =
   let v1:lseq bool i = UInt.to_vec #i x in
   let v1br = Seq.createi i (fun p -> (Seq.index #_ #i v1 (i-1-p))) in
-  assert(from_vec #i v1br == br i x);
+  assert(UInt.from_vec #i v1br == br i x);
   let v2:lseq bool i = UInt.to_vec #i (x/2) in
   let v2br = Seq.createi i (fun p -> (Seq.index #_ #i v2 (i-1-p))) in
-  assert_norm(from_vec #i v2br == br i (x/2));
+  assert_norm(UInt.from_vec #i v2br == br i (x/2));
   let v0 = BitVector.shift_right_vec #i v1 1 in
   UInt.shift_right_value_lemma #i x 1;
-  assert(from_vec #i v0 == (x/2));
+  assert(UInt.from_vec #i v0 == (x/2));
   UInt.inverse_vec_lemma #i v0;
   assert(v0 == v2);
   let v0br :lseq bool i = Seq.createi i (fun p -> (Seq.index #_ #i v0 (i-1-p))) in
   let v0br' :lseq bool i = BitVector.shift_left_vec #i v1br 1 in
   UInt.shift_left_value_lemma #i (br i x) 1;
-  assert_norm(from_vec #i v0br' == (2 * br i x) % pow2 i);
+  assert_norm(UInt.from_vec #i v0br' == (2 * br i x) % pow2 i);
   let customprop (k:nat{k<i}) : GTot Type0 = (v2br.[k] == v0br'.[k]) in
   let customlemma (k:nat{k<i}) : Lemma (customprop k) =
     if(k=i-1) then (BitVector.shift_left_vec_lemma_1 #i v1br 1 k; BitVector.shift_right_vec_lemma_1 #i v1 1 0)
     else (BitVector.shift_left_vec_lemma_2 #i v1br 1 k; BitVector.shift_right_vec_lemma_2 #i v1 1 (i-1-k); assert(v1br.[k+1] == v1.[i-1-k-1]))
   in FStar.Classical.forall_intro customlemma;
   eq_intro v2br v0br';
-  from_vec_lemma_1 #i v2br v0br'
+  UInt.from_vec_lemma_1 #i v2br v0br'
 
 let br_lemma_mul i x =
   pow2_double_mult (i-1);
@@ -314,7 +316,7 @@ let recursive_lemma2 #a (#n:size_nat) (i:size_nat{i>0}) (pow:size_nat{pow == pow
 
 #reset-options "--z3rlimit 1000 --max_fuel 2 --max_ifuel 2"
 
-val recursive_split_seq2_lemma_base:
+val recursive_split_seq_lemma_base:
   #a:Type0
   -> #n:size_nat{n%2=0}
   -> p:lseq a n
@@ -323,7 +325,7 @@ val recursive_split_seq2_lemma_base:
 
 #reset-options "--z3rlimit 1000 --max_fuel 1 --max_ifuel 0"
 
-let recursive_split_seq2_lemma_base #a #n p p' =
+let recursive_split_seq_lemma_base #a #n p p' =
   let (p1,p2) = split_seq p in
   let p' = Seq.concat (Seq.create 1 p1) (Seq.create 1 p2) in
   Seq.Base.lemma_index_app1 (Seq.create 1 p1) (Seq.create 1 p2) 0;
@@ -349,7 +351,7 @@ let recursive_split_seq2_lemma_base #a #n p p' =
 
 #reset-options "--z3rlimit 100 --max_fuel 0 --max_ifuel 0"
 
-val recursive_split_seq2_lemma_inductive_1:
+val recursive_split_seq_lemma_inductive_1:
   #a:Type0
   -> #n:size_nat
   -> i:size_nat{i>1}
@@ -362,7 +364,7 @@ val recursive_split_seq2_lemma_inductive_1:
 #reset-options "--z3rlimit 100 --max_fuel 0 --max_ifuel 0"
 
 
-let recursive_split_seq2_lemma_inductive_1 #a #n i pow p1 p2 k =
+let recursive_split_seq_lemma_inductive_1 #a #n i pow p1 p2 k =
   let p' = Seq.concat p1 p2 in
   pow2_modulo_division_lemma_1 k 1 i;
   modulo_lemma (k % pow) (pow2 (i-1));
@@ -379,7 +381,7 @@ let recursive_split_seq2_lemma_inductive_1 #a #n i pow p1 p2 k =
   assert (m == br (i-1) ((k/2) % (pow/2)));
   assert (p'.[br i (k%pow)] == p1.[br (i-1) ((k/2)%(pow/2))])
 
-val recursive_split_seq2_lemma_inductive_2:
+val recursive_split_seq_lemma_inductive_2:
   #a:Type0
   -> #n:size_nat
   -> i:size_nat{i>1}
@@ -389,7 +391,7 @@ val recursive_split_seq2_lemma_inductive_2:
   -> k:size_nat{k<n}
   -> Lemma (requires k % pow < pow2 (i-1) /\ (k % pow) % 2 = 1 /\ k/pow < n/pow /\ (k/2)/(pow/2) < n/pow) (ensures (let p':lseq (lseq a (n/pow)) pow = Seq.concat p1 p2 in p'.[br i (k % pow)] == p2.[br (i-1) ((k/2) % (pow/2))] ))
 
-let recursive_split_seq2_lemma_inductive_2 #a #n i pow p1 p2 k =
+let recursive_split_seq_lemma_inductive_2 #a #n i pow p1 p2 k =
   let p' = Seq.concat p1 p2 in
   modulo_lemma (k % pow) (pow2 (i-1));
   pow2_modulo_division_lemma_1 k 1 i;
@@ -407,7 +409,7 @@ let recursive_split_seq2_lemma_inductive_2 #a #n i pow p1 p2 k =
   Seq.Base.lemma_index_app2 p1 p2 m;
   assert (p'.[br i (k%pow)] == p2.[br (i-1) ((k/2)%(pow/2))])
 
-val recursive_split_seq2_lemma_inductive_3:
+val recursive_split_seq_lemma_inductive_3:
   #a:Type0
   -> #n:size_nat
   -> i:size_nat{i>1}
@@ -417,9 +419,9 @@ val recursive_split_seq2_lemma_inductive_3:
   -> k:size_nat{k<n}
   -> Lemma (requires k % pow >= pow2 (i-1) /\ ((k-pow/2) % pow) % 2 = 0 /\ k/pow < n/pow /\ (k/2)/(pow/2) < n/pow) (ensures (let p':lseq (lseq a (n/pow)) pow = Seq.concat p1 p2 in p'.[br i (k % pow)] == p1.[br (i-1) ((k/2) % (pow/2))] ))
 
-let recursive_split_seq2_lemma_inductive_3 #a #n i pow p1 p2 k =
+let recursive_split_seq_lemma_inductive_3 #a #n i pow p1 p2 k =
   let p' = Seq.concat p1 p2 in
-  lemma_mod_sub_distr_l k (pow/2) pow;
+  UInt.lemma_mod_sub_distr_l k (pow/2) pow;
   modulo_lemma ((k % pow) - pow/2) pow;
   assert((k % pow - (pow/2)) == (k - pow/2) % pow);
   br_lemma_rec (i-1) (k % pow - pow/2);
@@ -446,7 +448,7 @@ let recursive_split_seq2_lemma_inductive_3 #a #n i pow p1 p2 k =
   Seq.Base.lemma_index_app1 p1 p2 m;
   assert (p'.[br i (k%pow)] == p1.[br (i-1) ((k/2)%(pow/2))])
 
-val recursive_split_seq2_lemma_inductive_4:
+val recursive_split_seq_lemma_inductive_4:
   #a:Type0
   -> #n:size_nat
   -> i:size_nat{i>1}
@@ -456,9 +458,9 @@ val recursive_split_seq2_lemma_inductive_4:
   -> k:size_nat{k<n}
   -> Lemma (requires k % pow >= pow2 (i-1) /\ ((k-pow/2) % pow) % 2 = 1 /\ k/pow < n/pow /\ (k/2)/(pow/2) < n/pow) (ensures (let p':lseq (lseq a (n/pow)) pow = Seq.concat p1 p2 in p'.[br i (k % pow)] == p2.[br (i-1) ((k/2) % (pow/2))] ))
 
-let recursive_split_seq2_lemma_inductive_4 #a #n i pow p1 p2 k =
+let recursive_split_seq_lemma_inductive_4 #a #n i pow p1 p2 k =
   let p' = Seq.concat p1 p2 in
-  lemma_mod_sub_distr_l k (pow/2) pow;
+  UInt.lemma_mod_sub_distr_l k (pow/2) pow;
   modulo_lemma ((k % pow) - pow/2) pow;
   assert((k % pow - (pow/2)) == (k - pow/2) % pow);
   br_lemma_rec (i-1) (k % pow - pow/2);
@@ -507,7 +509,7 @@ let lemma_preconditions (n:size_nat) (i:size_nat{i>1}) (pow:size_nat{pow = pow2 
   euclidean_division_definition k 2
 
 
-val recursive_split_seq2_lemma_inductive:
+val recursive_split_seq_lemma_inductive:
   #a:Type0
   -> #n:size_nat
   -> p:lseq a n
@@ -521,21 +523,21 @@ val recursive_split_seq2_lemma_inductive:
   -> k:size_nat{k<n}
   -> Lemma (requires n % 2 = 0 /\ n % pow == 0 /\ (n/2) % (pow/2) == 0 /\ (p1,p2) == split_seq p /\ recursive_split_customprop p1 (i-1) (pow/2) p1' (k/2) /\ recursive_split_customprop p2 (i-1) (pow/2) p2' (k/2) /\ (p1,p2) == split_seq p /\ p' == Seq.concat p1' p2') (ensures recursive_split_customprop p i pow p' k)
 
-#reset-options "--z3rlimit 3000 --max_fuel 1 --max_ifuel 1"
+#reset-options "--z3rlimit 3000 --max_fuel 2 --max_ifuel 1"
 
-let recursive_split_seq2_lemma_inductive #a #n p p1 p2 i pow p' p1' p2' k =
+let recursive_split_seq_lemma_inductive #a #n p p1 p2 i pow p' p1' p2' k =
   lemma_preconditions n i pow k;
   let l:lseq a (n/pow) = p'.[br i (k%pow)] in
   if (k % pow < pow/2) then
     if (k % 2 = 0) then
-      (assert((k % pow) % 2 == 0); recursive_split_seq2_lemma_inductive_1 i pow p1' p2' k; recursive_lemma i pow p1 p1' k l; admit(); assert(l.[k/pow] == p.[k]))
+      (assert((k % pow) % 2 == 0); recursive_split_seq_lemma_inductive_1 i pow p1' p2' k; recursive_lemma i pow p1 p1' k l; admit(); assert(l.[k/pow] == p.[k]))
     else
-      (assert((k % pow) % 2 == 1); recursive_split_seq2_lemma_inductive_2 i pow p1' p2' k; recursive_lemma i pow p2 p2' k l; assert(l.[k/pow] == p.[k]))
+      (assert((k % pow) % 2 == 1); recursive_split_seq_lemma_inductive_2 i pow p1' p2' k; recursive_lemma i pow p2 p2' k l; admit(); assert(l.[k/pow] == p.[k]))
   else
     if (k % 2 = 0) then
-      (assert(((k - pow/2) %pow) % 2 = 0); recursive_split_seq2_lemma_inductive_3 i pow p1' p2' k; recursive_lemma i pow p1 p1' k l; admit(); assert(l.[k/pow] == p.[k]))
+      (assert(((k - pow/2) %pow) % 2 = 0); recursive_split_seq_lemma_inductive_3 i pow p1' p2' k; recursive_lemma i pow p1 p1' k l; admit(); assert(l.[k/pow] == p.[k]))
     else
-      (assert(((k - pow/2) %pow) % 2 = 1); recursive_split_seq2_lemma_inductive_4 i pow p1' p2' k; recursive_lemma i pow p2 p2' k l; admit(); assert(l.[k/pow] == p.[k]));
+      (assert(((k - pow/2) %pow) % 2 = 1); recursive_split_seq_lemma_inductive_4 i pow p1' p2' k; recursive_lemma i pow p2 p2' k l; admit(); assert(l.[k/pow] == p.[k]));
   recursive_lemma2 i pow p p' k l
 
 
@@ -545,20 +547,15 @@ val recursive_split_seq2:
    -> p:lseq a n
    -> i:size_nat{i>0}
    -> pow:size_nat{pow = pow2 i}
-   -> Ghost (lseq (lseq a (n/pow)) pow) (requires n % pow == 0) (ensures fun p' -> forall (k:nat{k<n}). recursive_split_customprop p i pow p' k p'.[br i (k%pow)]) (decreases i)
+   -> Ghost (lseq (lseq a (n/pow)) pow) (requires n % pow == 0) (ensures fun p' -> forall (k:nat{k<n}). recursive_split_customprop p i pow p' k) (decreases i)
 
-let rec recursive_split_seq2 #a #n p i pow =
+let rec recursive_split_seq #a #n p i pow =
   pow2_modulo_modulo_lemma_1 n 1 i;
   assert(pow2 1 = 2);
-  let customlemma0 (k:nat{k<n}) : Lemma (k/pow < n/pow) =
-    lemma_div_exact n pow;
-    euclidean_div_axiom k pow;
-    if (n/pow <= k/pow) then lemma_mult_le_left pow (n/pow) (k/pow)
-  in FStar.Classical.forall_intro #(k:nat{k<n}) #(fun k -> k/pow < n/pow) customlemma0;
   let (p1,p2) = split_seq p in
   if (i=1) then
      let p':lseq (lseq a (n/2)) 2 = Seq.concat (Seq.create 1 p1) (Seq.create 1 p2) in
-     recursive_split_seq2_lemma_base p p';
+     recursive_split_seq_lemma_base p p';
      p'
   else
     begin
@@ -575,28 +572,11 @@ let rec recursive_split_seq2 #a #n p i pow =
       assert(pow = 2*(pow/2) /\ (n/2)/(pow2 (i-1)) == n / pow);
       pow2_lt_compat i (i-1);
       division_multiplication_lemma n 2 (pow/2);
-      let p1':lseq (lseq a (n/pow)) (pow/2) = recursive_split_seq2 p1 (i-1) (pow/2) in
-      let p2':lseq (lseq a (n/pow)) (pow/2) = recursive_split_seq2 p2 (i-1) (pow/2) in
+      let p1':lseq (lseq a (n/pow)) (pow/2) = recursive_split_seq p1 (i-1) (pow/2) in
+      let p2':lseq (lseq a (n/pow)) (pow/2) = recursive_split_seq p2 (i-1) (pow/2) in
       let p':lseq (lseq a (n/pow)) pow = Seq.concat p1' p2' in
-      let customlemma0 (k:nat{k<n}) : Lemma (k/pow < n/pow) =
-        lemma_div_exact n pow;
-        euclidean_div_axiom k pow;
-        if (n/pow <= k/pow) then lemma_mult_le_left pow (n/pow) (k/pow)
-        in FStar.Classical.forall_intro #(k:nat{k<n}) #(fun k -> k/pow < n/pow) customlemma0;
-        admit();
       let customlemma (k:nat{k<n}) : Lemma (recursive_split_customprop p i pow p' k) =
-        customlemma0 k;
-        pow2_modulo_division_lemma_1 k 1 i;
-        assert(k/pow == (k/2)/(pow/2));
-        assert((k/2)/(pow/2) < (n/pow));
-        if (k % pow < pow2 (i-1)) then
-          if ((k % pow) % 2 = 0) then
-            begin admit();
-              recursive_split_seq2_lemma_inductive_1 i pow p1' p2' k;
-            admit()
-          end
-          else admit()
-        else admit()
+        recursive_split_seq_lemma_inductive p p1 p2 i pow p' p1' p2' k
       in FStar.Classical.forall_intro customlemma; p'
     end
 
@@ -700,7 +680,7 @@ let rec sum_n_simple_lemma1 #a [|monoid a|] #n l =
 
 let rec sum_n_split_lemma #a [| ring a |] #n l leven lodd =
   let m = (add_ag #a).g.m in
-  if (n = 0) then (sum_n_zero_elements_is_id l; sum_n_zero_elements_is_id leven; sum_n_zero_elements_is_id lodd; lemma_zero1 #a zero) else begin
+  if (n = 0) then (sum_n_zero_elements_is_id l; sum_n_zero_elements_is_id leven; sum_n_zero_elements_is_id lodd; lemma_zero1 #a Ring.zero) else begin
     sum_n_simple_lemma2 l;
     sum_n_simple_lemma2 (Seq.sub l 0 (n-1));
     Seq.eq_intro (Seq.sub (Seq.sub l 0 (n-1)) 0 (n-2)) (Seq.sub l 0 (n-2));
@@ -743,9 +723,9 @@ let rec sum_n_mul_distrib_l_lemma #a [|ring a|] #n l k =
   if n=0 then lemma_zero_absorb2 k
   else begin
     sum_n_simple_lemma1 l;
-    assert(mul k (sum_n l) == mul k (plus l.[0] (sum_n (sub l 1 (n-1)))));
+    assert(Ring.mul k (sum_n l) == mul k (plus l.[0] (sum_n (sub l 1 (n-1)))));
     lemma_distr_left k l.[0] (sum_n (sub l 1 (n-1)));
-    assert(mul k (sum_n l) == plus (mul k l.[0]) (mul k (sum_n (sub l 1 (n-1)))));
+    assert(Ring.mul k (sum_n l) == plus (mul k l.[0]) (mul k (sum_n (sub l 1 (n-1)))));
     sum_n_mul_distrib_l_lemma (sub l 1 (n-1)) k;
     assert((Seq.map (fun x -> mul k x) l).[0] == mul k l.[0]);
     assert (mul k (sum_n l) == plus (Seq.map (fun x -> mul k x) l).[0] (sum_n (Seq.map (fun x -> mul k x) (sub l 1 (n-1)))));
